theories/iris/examples/effects/generator_client.v
@@ -10,6 +10,7 @@ From iris.algebra Require Import list excl_auth.
 From Wasm Require Import type_checker_reflects_typing.
 From Wasm.iris.rules Require Export iris_rules iris_example_helper.
 From Wasm.iris.host Require Export iris_host.
+From Wasm.iris.examples.effects Require Import generator.
 From Wasm.iris.examples.effects Require Import generator_module.
 
 
@@ -40,84 +41,62 @@ Definition sum_until_client_0:=
 Definition sum_until_client_neg :=
   [BI_const $ xx (-4294967293); BI_call 0].
 
-Definition sum_until_client_100_host generator_exp_addr sum_until_exp_addr mod_addr :=
-  [ ID_instantiate [ generator_exp_addr; sum_until_exp_addr ] mod_addr [];
-    H_invoke sum_until_exp_addr [xx 100]
-  ].
+Section GeneratorClient.
+  Context `{!wasmG Σ, !hvisG Σ, !hmsG Σ, !hasG Σ}.
+  Context `{!inG Σ (excl_authR (listO (leibnizO i32)))}.
+
+  Definition sum_until_client generator_exp_addr sum_until_exp_addr mod_addr n :=
+    [ ID_instantiate [ generator_exp_addr; sum_until_exp_addr ] mod_addr [];
+H_invoke sum_until_exp_addr [VAL_int32 n]
+    ].
 
   Notation "{{{{ P }}}} es {{{{ v , Q }}}}" :=
     (□ ∀ Φ, P -∗ (∀ v, Q -∗ Φ v) -∗ WP (es : host_expr) @ NotStuck ; ⊤ {{ v, Φ v }})%I (at level 50).
 
 
-  Lemma instantiate_client naturals_exp_addr sum_until_exp_addr mod_addr :
+  Lemma instantiate_client naturals_exp_addr sum_until_exp_addr mod_addr n :
     ⊢ {{{{
         mod_addr ↪[mods] generator_module ∗
         (∃ exp1, naturals_exp_addr ↪[vis] exp1) ∗
         (∃ exp2, sum_until_exp_addr ↪[vis] exp2)
       }}}}
-      (sum_until_client_100_host naturals_exp_addr sum_until_exp_addr mod_addr : host_expr)
-      {{{{ x, ⌜ exists a b, x = (immHV [VAL_num (xx a); VAL_num (xx b)], empty_frame) /\ (a = 1 -> b = 42) ⌝ }}}}.
-Section sum_until_clients_spec.
-
-  Context `{!wasmG Σ}.
-
-  Lemma sum_until_100 addr_naturals addr_sum_until cl_sum_until cl_naturals f :
-    N.of_nat addr_sum_until ↦[wf] cl_sum_until -∗
-    N.of_nat addr_naturals ↦[wf] cl_naturals -∗
-    EWP sum_until_client_100 UNDER f
-      {{ v ; f', ⌜f = f' ∧ v = immV [VAL_num $ xx 5050]⌝ }}.
+        ((sum_until_client naturals_exp_addr sum_until_exp_addr mod_addr n, [], empty_frame) : host_expr)
+      {{{{ w, ⌜w = (immHV [VAL_num (VAL_int32 $ Sum_until_i32 n)], empty_frame)⌝ }}}}.
   Proof.
-    iIntros "Haddr_sum_until Haddr_naturals #Htag".
-    iApply (ewp_wand with "[-] []").
-    - iApply (sum_until_spec_proof with "[Haddr_sum_until] [Haddr_naturals]"); done.
-    - iIntros (?? [-> ->]).
-      iPureIntro.
-      split; first done.
-      unfold Sum_until_i32.
-      repeat f_equal.
-      replace (xy (yx 100)) with (100); last done.
-      repeat rewrite big_nat_recl //=.
-      rewrite big_geq; done.
+    iIntros "!>" (Φ) "(Hmod & Hexp1 & Hexp2 ) HΦ".
+
+    (* instantiate generator module *)
+    iApply (wp_seq_host_nostart with "[] Hmod [Hexp1 Hexp2]").
+    done. done.
+    2:{
+      iIntros "Hmod".
+      iApply (instantiate_generator with "[$Hmod $Hexp1 $Hexp2]").
+      iIntros (x) "(-> & Hmod & H)".
+      iFrame.
+      instantiate (1 := λ v, (⌜ v = (immHV [], empty_frame) ⌝ ∗ _)%I).
+      iSplit; first done.
+      iExact "H".
+    }
+    by iIntros (?) "[% _]".
+    iIntros (w f) "(%Heq & %addr_naturals & %addr_sum_until & %name_naturals & %name_sum_until & %cl_naturals & %cl_sum_until & Hexp1 & Hexp2 & %Htypenaturals & %Htypesum_until & Hwfnaturals & Hwfsum_until & #Hspecs) Hmod".
+    iDestruct (pointsto_ne with "Hwfnaturals Hwfsum_until") as %Hne.
+    inversion Heq; subst. clear Heq.
+
+    replace [] with (v_to_e_list []); last done.
+    iApply (wp_invoke_host with "[$] [$Hwfsum_until]").
+    done.
+    done.
+    iIntros "!> Hexpsum_until Hwfsum_until".
+
+    iApply wp_lift_wasm.
+
+    (* Prove the specification of sum_until *)
+    simpl.
+    iApply (ewp_wand with "[-HΦ]").
+    iApply ("Hspecs" with "[Hwfsum_until] [Hwfnaturals]"); done.
+    iIntros (?? [<- ->]); simpl.
+    iApply wp_value; first done.
+    by iApply "HΦ".
   Qed.
 
-  Lemma sum_until_0 addr_naturals addr_sum_until addr_tag f :
-    N.of_nat addr_sum_until ↦[wf] closure_sum_until addr_naturals addr_sum_until addr_tag -∗
-    N.of_nat addr_naturals ↦[wf] closure_naturals addr_naturals addr_tag -∗
-    N.of_nat addr_tag ↦□[tag] tag_type -∗
-    EWP [AI_const $ VAL_num $ VAL_int32 $ yx 0; AI_invoke addr_sum_until] UNDER f
-      {{ v ; f', ⌜f = f' ∧ v = immV [VAL_num $ VAL_int32 $ yx 0]⌝ }}.
-  Proof.
-    iIntros "Haddr_sum_until Haddr_naturals #Htag".
-    iApply (ewp_wand with "[-] []").
-    - iApply (sum_until_spec_proof with "[Haddr_sum_until] [Haddr_naturals]"); done.
-    - iIntros (?? [-> ->]).
-      iPureIntro.
-      split; first done.
-      unfold Sum_until_i32.
-      repeat f_equal.
-      replace (xy (yx 0)) with (0); last done.
-      repeat rewrite big_nat_recl //=.
-      rewrite big_geq; done.
-  Qed.
-
-  Lemma sum_until_3_neg addr_naturals addr_sum_until addr_tag f :
-    N.of_nat addr_sum_until ↦[wf] closure_sum_until addr_naturals addr_sum_until addr_tag -∗
-    N.of_nat addr_naturals ↦[wf] closure_naturals addr_naturals addr_tag -∗
-    N.of_nat addr_tag ↦□[tag] tag_type -∗
-    EWP [AI_const $ VAL_num $ VAL_int32 $ yx (-4294967293); AI_invoke addr_sum_until] UNDER f
-      {{ v ; f', ⌜f = f' ∧ v = immV [VAL_num $ VAL_int32 $ yx 6]⌝ }}.
-  Proof.
-    iIntros "Haddr_sum_until Haddr_naturals #Htag".
-    iApply (ewp_wand with "[-] []").
-    - iApply (sum_until_spec_proof with "[Haddr_sum_until] [Haddr_naturals]"); done.
-    - iIntros (?? [-> ->]).
-      iPureIntro.
-      split; first done.
-      unfold Sum_until_i32.
-      repeat f_equal.
-      replace (xy (yx (-4294967293))) with (3); last done.
-      repeat rewrite big_nat_recl //=.
-      rewrite big_geq; done.
-  Qed.
-
-End sum_until_spec.
+End GeneratorClient.
